WFNOMutationEXP.v
@@ -103,4 +103,32 @@ Proof.
   unfold vpa_assignability in Hvpa_assignable.
   destruct a eqn: Heq_a; destruct (rqtype (rt_type o)) eqn: Heq_rq; destruct (sqtype Tx) eqn: Heq_sq; try discriminate.
   destruct qcontext eqn: Heq_qc; try easy.
+  -
+  rename sΓ' into sΓ.
+  destruct (extract_receiver_from_wf_config CT sΓ rΓ h Hwf) as [iot [qcontext [Hget_iot[Hiot_dom Hqcontext]]]].
+  unfold wf_r_config in Hwf.
+  destruct Hwf as [Hclass [Hheap [Hrenv [Hsenv [Hlen Hcorr]]]]].
+  specialize (Hcorr iot qcontext Hget_iot Hqcontext).
+  have Htype_x : static_getType sΓ x = Some Tx by exact Hget_x.
+  have Hxdom: x < dom sΓ by (apply static_getType_dom in Htype_x; auto).
+  specialize (Hcorr x Hxdom Tx Htype_x).
+  rewrite Hgetval_x in Hcorr.
+  unfold wf_r_typable in Hcorr.
+  unfold r_type in Hcorr.
+  rewrite Hgetobj in Hcorr.
+  destruct Hcorr as [Hbase Hqualifer].
+  assert (sf_assignability_rel CT (rctype (rt_type o)) f a0).
+  {
+    eapply sf_assignability_subtyping; eauto.
+  }
+  assert (a0 = a).
+  {
+    eapply sf_assignability_deterministic_rel; eauto.
+  }
+  subst a0.
+  rename Hassignable into Hvpa_assignable.
+  unfold runtime_vpa_assignability in Hvpa_final.
+  unfold vpa_assignability_concret_imm in Hvpa_assignable.
+  destruct a eqn: Heq_a; destruct (rqtype (rt_type o)) eqn: Heq_rq; destruct (sqtype Tx) eqn: Heq_sq; try discriminate.
+  destruct qcontext eqn: Heq_qc; try easy.
 Qed.
